\documentclass[border=2pt]{standalone}
\usepackage{amsmath}
\usepackage{amssymb}

\begin{document}

\begin{tabular}{|c|c|c|c|c|c|c|}
\hline \multicolumn{2}{|c|}{\textbf{Space frame} } & \multicolumn{3}{c|}{Transformation} & \multicolumn{2}{c|}{\textbf{Body frame} }\\
\hline  \begin{tabular}{@{}c@{}}
\textbf{Vector}\\
 (Cartesian space)
\end{tabular}  &  \begin{tabular}{@{}c@{}}
\textbf{Lie algebra}\\
 (Tangent space)
\end{tabular}  &  from \ensuremath{\left\{b\right\}} to \ensuremath{\left\{s\right\}} &  Adjoint matrix  &  from \ensuremath{\left\{s\right\}} to \ensuremath{\left\{b\right\}}  &  \begin{tabular}{@{}c@{}}
\textbf{Lie algebra}\\
 (Tangent space)
\end{tabular}  &  \begin{tabular}{@{}c@{}}
\textbf{Vector}\\
 (Cartesian space)
\end{tabular} \\
\hline  \begin{tabular}{@{}c@{}}
Spatial angular velocity\\
\ensuremath{\boldsymbol{\omega}_{s}}
\end{tabular}  & \ensuremath{\begin{array}{rl}
\dot{\mathbf{R}}\mathbf{R}^{-1} & =\left[\boldsymbol{\omega}_{s}\times\right]\\
\dot{\mathbf{R}} & =\left[\boldsymbol{\omega}_{s}\times\right]\mathbf{R}\\
\mathbf{R} & =\exp\left(\left[\boldsymbol{\omega}_{s}\times\right]\cdot\Delta t\right)
\end{array}}  & \ensuremath{\begin{array}{rl}
\left[\boldsymbol{\omega}_{s}\times\right] & =\mathbf{R}\left[\boldsymbol{\omega}_{b}\times\right]\mathbf{R}^{-1}\\
 & =\left[\left(\mathbf{R}\boldsymbol{\omega}_{b}\right)\times\right]\\
\boldsymbol{\omega}_{s} & =\mathbf{R}\boldsymbol{\omega}_{b}
\end{array}}  & \ensuremath{\begin{array}{rl}
\left[\mathrm{Ad}_{\mathbf{R}}\right] & =\mathbf{R}\\
\ensuremath{\boldsymbol{\omega}_{s}} & =\mathbf{R}\boldsymbol{\omega}_{b}\\
\left[\mathrm{Ad}_{\mathbf{R}^{-1}}\right] & =\mathbf{R}^{-1}\\
\boldsymbol{\omega}_{b} & =\mathbf{R}^{-1}\boldsymbol{\omega}_{s}
\end{array}} & \ensuremath{\begin{array}{rl}
\left[\boldsymbol{\omega}_{b}\times\right] & =\mathbf{R}^{-1}\left[\boldsymbol{\omega}_{s}\times\right]\mathbf{R}\\
 & =\left[\left(\mathbf{R}^{-1}\boldsymbol{\omega}_{s}\right)\times\right]\\
\boldsymbol{\omega}_{b} & =\mathbf{R}^{-1}\boldsymbol{\omega}_{s}
\end{array}} & \ensuremath{\begin{array}{rl}
\mathbf{R}^{-1}\dot{\mathbf{R}} & =\left[\boldsymbol{\omega}_{b}\times\right]\\
\ensuremath{\dot{\mathbf{R}}} & =\mathbf{R}\left[\boldsymbol{\omega}_{b}\times\right]\\
\mathbf{R}^{-1} & =\exp\left(\left[\boldsymbol{\omega}_{b}\times\right]\cdot\Delta t\right)
\end{array}} &  \begin{tabular}{@{}c@{}}
Body angular velocity\\
\ensuremath{\boldsymbol{\omega}_{b}}
\end{tabular} \\
\hline  \begin{tabular}{@{}c@{}}
Spatial velocity\\
\ensuremath{\boldsymbol{\mathcal{V}}_{s}=\left[\begin{array}{c}
\boldsymbol{\omega}_{s}\\
\mathbf{v}_{s}
\end{array}\right]}
\end{tabular}  & \ensuremath{\begin{array}{rl}
\dot{\mathbf{T}}\mathbf{T}^{-1} & =\left[\boldsymbol{\mathcal{V}}_{s}^{\wedge}\right]\\
 & =\left[\begin{array}{c|c}
\left[\boldsymbol{\omega}_{s}\times\right] & \mathbf{v}_{s}\\
\hline \mathbf{0}^{\mathrm{T}} & 0
\end{array}\right]\\
\dot{\mathbf{T}} & =\left[\boldsymbol{\mathcal{V}}_{s}^{\wedge}\right]\mathbf{T}\\
\mathbf{T} & =\exp\left(\left[\boldsymbol{\mathcal{V}}_{s}^{\wedge}\right]\cdot\Delta t\right)
\end{array}} & \ensuremath{\begin{array}{rl}
\ensuremath{\left[\boldsymbol{\mathcal{V}}_{s}^{\wedge}\right]} & =\mathbf{T}\left[\boldsymbol{\mathcal{V}}_{b}^{\wedge}\right]\mathbf{T}^{-1}\\
\boldsymbol{\mathcal{V}}_{s} & =\left[\mathrm{Ad}_{\mathbf{T}}\right]\boldsymbol{\mathcal{V}}_{b}
\end{array}} & \ensuremath{\begin{array}{rl}
\left[\mathrm{Ad}_{\mathbf{T}}\right] & =\left[\begin{array}{cc}
\mathbf{R} & \mathbf{0}\\
\left[\mathbf{r}\times\right]\mathbf{R} & \mathbf{R}
\end{array}\right]\\
\ensuremath{\boldsymbol{\mathcal{V}}_{s}} & =\left[\mathrm{Ad}_{\mathbf{T}}\right]\boldsymbol{\mathcal{V}}_{b}\\
\left[\mathrm{Ad}_{\mathbf{T}^{-1}}\right] & =\left[\begin{array}{cc}
\mathbf{R}^{-1} & \mathbf{0}\\
-\mathbf{R}^{-1}\left[\mathbf{r}\times\right] & \mathbf{R}^{-1}
\end{array}\right]\\
\boldsymbol{\mathcal{V}}_{b} & =\left[\mathrm{Ad}_{\mathbf{T}^{-1}}\right]\boldsymbol{\mathcal{V}}_{s}
\end{array}} & \ensuremath{\begin{array}{rl}
\ensuremath{\left[\boldsymbol{\mathcal{V}}_{b}^{\wedge}\right]} & =\mathbf{T}^{-1}\left[\boldsymbol{\mathcal{V}}_{s}^{\wedge}\right]\mathbf{T}\\
\boldsymbol{\mathcal{V}}_{b} & =\left[\mathrm{Ad}_{\mathbf{T}^{-1}}\right]\boldsymbol{\mathcal{V}}_{s}
\end{array}} & \ensuremath{\begin{array}{rl}
\mathbf{T}^{-1}\dot{\mathbf{T}} & =\left[\boldsymbol{\mathcal{V}}_{b}^{\wedge}\right]\\
 & =\left[\begin{array}{c|c}
\left[\boldsymbol{\omega}_{b}\times\right] & \mathbf{v}_{b}\\
\hline \mathbf{0}^{\mathrm{T}} & 0
\end{array}\right]\\
\dot{\mathbf{T}} & =\mathbf{T}\left[\boldsymbol{\mathcal{V}}_{b}^{\wedge}\right]\\
\mathbf{T}^{-1} & =\exp\left(\left[\boldsymbol{\mathcal{V}}_{b}^{\wedge}\right]\cdot\Delta t\right)
\end{array}} &  \begin{tabular}{@{}c@{}}
Body velocity\\
\ensuremath{\boldsymbol{\mathcal{V}}_{b}=\left[\begin{array}{c}
\boldsymbol{\omega}_{b}\\
\mathbf{v}_{b}
\end{array}\right]}
\end{tabular} \\
\hline
\end{tabular}

\end{document}
